reorganization: move more things into BaseConversion

src/Experiments/SimplyTypedArithmetic.v
@@ -595,30 +595,6 @@ Section mod_ops.
   Qed.
 End mod_ops.
 
-Module BaseConversion.
-  Import Positional.
-  Section BaseConversion.
-    Context (sw dw : nat -> Z) (* source/destination weight functions *)
-            (dw_0 : dw 0%nat = 1)
-            (dw_nz : forall i, dw i <> 0).
-    Context (dw_divides : forall i : nat, dw (S i) / dw i > 0).
-
-    Definition convert_bases (sn dn : nat) (p : list Z) : list Z :=
-      let p' := Positional.from_associational dw dn (Positional.to_associational sw sn p) in
-      chained_carries_no_reduce dw dn p' (seq 0 (pred dn)).
-
-    Lemma eval_convert_bases sn dn p :
-      (dn <> 0%nat) -> length p = sn ->
-      eval dw dn (convert_bases sn dn p) = eval sw sn p.
-    Proof.
-      cbv [convert_bases]; intros.
-      rewrite eval_chained_carries_no_reduce; auto using ZUtil.Z.positive_is_nonzero.
-      rewrite eval_from_associational; auto.
-    Qed.
-
-  End BaseConversion.
-End BaseConversion.
-
 Module Saturated.
   Section Weight.
     Context (weight : nat->Z)
@@ -640,7 +616,7 @@ Module Saturated.
                | _ => reflexivity
                end.
     Qed.
-    
+
     Lemma weight_multiples_full j i : (i <= j)%nat -> weight j mod weight i = 0.
     Proof.
       intros; replace j with (i + (j - i))%nat by omega.
@@ -714,7 +690,7 @@ Module Saturated.
       rewrite Z.mod_pull_div, Z.mul_div_eq' by auto using Z.gt_lt.
       repeat (f_equal; try omega).
     Qed.
-    
+
     Lemma add_mod_l_multiple a b n m:
       0 < n / m -> m <> 0 -> n mod m = 0 ->
       (a mod n + b) mod m = (a + b) mod m.
@@ -727,7 +703,7 @@ Module Saturated.
     Qed.
 
     Definition is_div_mod {T} (evalf : T -> Z) dm y n :=
-      evalf (fst dm) = y mod n /\ snd dm = y / n. 
+      evalf (fst dm) = y mod n /\ snd dm = y / n.
 
     Lemma is_div_mod_step {T} evalf1 evalf2 dm1 dm2 y1 y2 n1 n2 x :
       n1 > 0 ->
@@ -842,14 +818,14 @@ Module Columns.
                | _ => progress autorewrite with pull_Zmod pull_Zdiv zsimplify_fast
                | _ => progress autorewrite with list distr_length push_eval
                end.
-      
+
       Lemma flatten_column_mod fw (xs : list Z) :
         fst (flatten_column fw xs)  = sum xs mod fw.
       Proof.
         induction xs; simpl flatten_column; cbv [Let_In];
           repeat match goal with
                  | _ => rewrite IHxs
-                 | _ => progress push 
+                 | _ => progress push
                  end.
       Qed. Hint Rewrite flatten_column_mod : to_div_mod.
 
@@ -964,7 +940,7 @@ Module Columns.
       Hint Rewrite Positional.eval_zeros : push_eval.
       Hint Rewrite Positional.length_from_associational : distr_length.
       Hint Rewrite Positional.eval_add_to_nth using (solve [distr_length]): push_eval.
-      
+
       (* from_associational *)
       Definition from_associational n (p:list (Z*Z)) : list (list Z) :=
         List.fold_right (fun t ls =>
@@ -1062,7 +1038,7 @@ Module Rows.
                  | _ => progress distr_length
                  | _ => rewrite Positional.eval_snoc with (n:=n) by distr_length
                  | _ => progress autorewrite with cancel_pair push_eval push_map in *
-                 | _ => ring 
+                 | _ => ring
                  end.
         rewrite IHinp by distr_length.
         destruct x; cbn [hd tl]; rewrite ?sum_nil, ?sum_cons; ring.
@@ -1072,7 +1048,7 @@ Module Rows.
         length inp = n -> length (fst (extract_row inp)) = n.
       Proof. cbv [extract_row]; autorewrite with cancel_pair; distr_length. Qed.
       Hint Rewrite length_fst_extract_row : distr_length.
-      
+
       Lemma length_snd_extract_row n (inp : cols) :
         length inp = n -> length (snd (extract_row inp)) = n.
       Proof. cbv [extract_row]; autorewrite with cancel_pair; distr_length. Qed.
@@ -1084,7 +1060,7 @@ Module Rows.
       (* TODO: move to where list is defined *)
       Hint Rewrite @app_nil_l : list.
       Hint Rewrite <-@app_comm_cons: list.
- 
+
       Lemma max_column_size_nil : max_column_size nil = 0%nat.
       Proof. reflexivity. Qed. Hint Rewrite max_column_size_nil : push_max_column_size.
       Lemma max_column_size_cons col (inp : cols) :
@@ -1142,7 +1118,7 @@ Module Rows.
       Proof. apply eval_from_columns'_with_length. reflexivity. Qed.
       Hint Rewrite length_snd_from_columns' : distr_length.
       Lemma eval_from_columns' m st n :
-        (length (fst st) = n) -> 
+        (length (fst st) = n) ->
         eval n (snd (from_columns' m st)) = Columns.eval weight n (fst st) + eval n (snd st)
                                                                              - Columns.eval weight n (fst (from_columns' m st)).
       Proof. apply eval_from_columns'_with_length. Qed.
@@ -1191,7 +1167,7 @@ Module Rows.
 
       (* from associational *)
       Definition from_associational n (p : list (Z * Z)) := from_columns (Columns.from_associational weight n p).
-      
+
       Lemma eval_from_associational n p: (n <> 0%nat \/ p = nil) ->
                                          eval n (from_associational n p) = Associational.eval p.
       Proof.
@@ -1253,7 +1229,7 @@ Module Rows.
         rewrite <-nth_default_eq in *.
         autorewrite with push_nth_default in *.
         rewrite eq_nat_dec_refl in *.
-        congruence. 
+        congruence.
       Qed.
 
       Lemma from_associational_nonnil n p :
@@ -1334,7 +1310,7 @@ Module Rows.
           apply IHrow1; clear IHrow1; autorewrite with cancel_pair distr_length in *; try omega.
           eapply is_div_mod_step with (x := x1 + x2); try eassumption; push.
         Qed.
-        
+
         Lemma sum_rows_div_mod n row1 row2 :
           length row1 = n -> length row2 = n ->
           let eval := Positional.eval weight in
@@ -1373,7 +1349,7 @@ Module Rows.
                       = ((eval nm (row1' ++ row1) + eval nm (row2' ++ row2)) mod (weight (S i))) / (weight i).
         Proof.
           induction row1 as [|x1 row1]; destruct row2 as [|x2 row2]; intros; subst nm; push; [].
-          
+
           rewrite (app_cons_app_app _ row1'), (app_cons_app_app _ row2').
           apply IHrow1; clear IHrow1; push;
             repeat match goal with
@@ -1390,7 +1366,7 @@ Module Rows.
             push. rewrite add_mod_div_multiple by auto using Z.lt_le_incl.
             push. }
         Qed.
-        
+
         Lemma sum_rows_partitions row1: forall row2 n i,
             length row1 = n -> length row2 = n -> (i < n)%nat ->
             nth_default 0 (fst (sum_rows row1 row2)) i
@@ -1493,7 +1469,7 @@ Module Rows.
         (forall row, In row inp -> length row = n) ->
         length (fst (flatten' start_state inp)) = n.
       Proof. apply flatten'_div_mod_length. Qed.
-      Hint Rewrite length_flatten' : distr_length. 
+      Hint Rewrite length_flatten' : distr_length.
 
       Lemma length_flatten n inp :
         (forall row, In row inp -> length row = n) ->
@@ -1551,8 +1527,8 @@ Module Rows.
           match goal with H : context [nth_default _ (p ++ [ _ ])] |- _ =>
                           rewrite <-H by omega end.
         { autorewrite with push_nth_default natsimplify. reflexivity. }
-        { autorewrite with push_nth_default natsimplify. 
-          break_match; omega. } 
+        { autorewrite with push_nth_default natsimplify.
+          break_match; omega. }
       Qed.
 
       Lemma flatten_partitions' inp n :
@@ -1595,31 +1571,96 @@ Module Rows.
   End Rows.
 End Rows.
 
-Module MulConverted.
-  Section mul_converted.
-      Context (w w' : nat -> Z).
-      Context (w'_0 : w' 0%nat = 1)
-              (w'_nonzero : forall i, w' i <> 0)
-              (w'_positive : forall i, w' i > 0)
-              (w'_divides : forall i : nat, w' (S i) / w' i > 0).
-      Context (w_0 : w 0%nat = 1)
-              (w_nonzero : forall i, w i <> 0)
-              (w_positive : forall i, w i > 0)
-              (w_multiples : forall i, w (S i) mod w i = 0)
-              (w_divides : forall i : nat, w (S i) / w i > 0).
+Module BaseConversion.
+  Import Positional.
+  Section BaseConversion.
+    Context (sw dw : nat -> Z) (* source/destination weight functions *)
+            (dw_0 : dw 0%nat = 1)
+            (sw_0 : sw 0%nat = 1)
+            (dw_nz : forall i, dw i <> 0)
+            (sw_nz : forall i, sw i <> 0)
+            (sw_pos : forall i, sw i > 0)
+            (sw_multiples : forall i, sw (S i) mod sw i = 0)
+            (sw_divides : forall i, sw (S i) / sw i > 0)
+            (dw_divides : forall i, dw (S i) / dw i > 0).
 
-      (* TODO : move this stuff to BaseConversion *)
-        Definition to_associational n m p : list (Z * Z) :=
-          let p' := BaseConversion.convert_bases w w' n m p in
-          Positional.to_associational w' m p'.
+    Definition convert_bases (sn dn : nat) (p : list Z) : list Z :=
+      let p' := Positional.from_associational dw dn (Positional.to_associational sw sn p) in
+      chained_carries_no_reduce dw dn p' (seq 0 (pred dn)).
 
-        Definition from_associational idxs n (p : list (Z * Z)) : list Z :=
-          (* important not to use Positional.carry here; we don't want to accumulate yet *)
-          let p' := fold_right (fun i acc => Associational.carry (w' i) (w' (S i) / w' i) acc) p (rev idxs) in
-          fst (Rows.flatten w n (Rows.from_associational w n p')).
+    Lemma eval_convert_bases sn dn p :
+      (dn <> 0%nat) -> length p = sn ->
+      eval dw dn (convert_bases sn dn p) = eval sw sn p.
+    Proof.
+      cbv [convert_bases]; intros.
+      rewrite eval_chained_carries_no_reduce; auto using ZUtil.Z.positive_is_nonzero.
+      rewrite eval_from_associational; auto.
+    Qed.
 
-      (* takes in inputs in base w, converts to w', multiplies in that
-         format, converts to w again, then flattens. *)
+    Hint Rewrite
+         @Rows.eval_from_associational
+         @Associational.eval_carry
+         @Associational.eval_mul
+         @Positional.eval_to_associational
+         @eval_convert_bases using solve [auto using Z.positive_is_nonzero] : push_eval.
+
+    Ltac push_eval := intros; autorewrite with push_eval; auto with zarith.
+
+    (* convert from positional in one weight to the other, then to associational *)
+    Definition to_associational n m p : list (Z * Z) :=
+      let p' := convert_bases n m p in
+      Positional.to_associational dw m p'.
+
+    (* carry at specified indices in dw, then use Rows.flatten to convert to Positional with sw *)
+    Definition from_associational idxs n (p : list (Z * Z)) : list Z :=
+      (* important not to use Positional.carry here; we don't want to accumulate yet *)
+      let p' := fold_right (fun i acc => Associational.carry (dw i) (dw (S i) / dw i) acc) p (rev idxs) in
+      fst (Rows.flatten sw n (Rows.from_associational sw n p')).
+
+    Lemma eval_carries p idxs :
+      Associational.eval (fold_right (fun i acc => Associational.carry (dw i) (dw (S i) / dw i) acc) p idxs) =
+      Associational.eval p.
+    Proof. apply fold_right_invariant; push_eval. Qed.
+    Hint Rewrite eval_carries: push_eval.
+
+    Lemma eval_to_associational n m p :
+      m <> 0%nat -> length p = n ->
+      Associational.eval (to_associational n m p) = Positional.eval sw n p.
+    Proof. cbv [to_associational]; push_eval. Qed.
+    Hint Rewrite eval_to_associational using solve [push_eval; distr_length] : push_eval.
+
+    Lemma eval_from_associational idxs n p :
+      n <> 0%nat -> 0 <= Associational.eval p < sw n ->
+      Positional.eval sw n (from_associational idxs n p) = Associational.eval p.
+    Proof.
+      cbv [from_associational]; intros.
+      rewrite Rows.flatten_mod by eauto using Rows.length_from_associational.
+      push_eval.
+    Qed.
+    Hint Rewrite eval_from_associational using solve [push_eval; distr_length] : push_eval.
+
+    Lemma from_associational_partitions n idxs p  (_:n<>0%nat):
+      forall i, (i < n)%nat ->
+                nth_default 0 (from_associational idxs n p) i = (Associational.eval p) mod (sw (S i)) / sw i.
+    Proof.
+      intros; cbv [from_associational].
+      rewrite Rows.flatten_partitions with (n:=n) by (eauto using Rows.length_from_associational; omega).
+      push_eval.
+    Qed.
+
+    Lemma from_associational_eq n idxs p  (_:n<>0%nat):
+      from_associational idxs n p = Rows.partition sw n (Associational.eval p).
+    Proof.
+      intros. cbv [from_associational].
+      rewrite Rows.flatten_partitions' with (n:=n) by eauto using Rows.length_from_associational.
+      push_eval.
+    Qed.
+
+    (* carry chain that aligns terms in the intermediate weight with the final weight *)
+    Definition aligned_carries (log_dw_sw nout : nat)
+      := (map (fun i => ((log_dw_sw * (i + 1)) - 1))%nat (seq 0 nout)).
+
+    Section mul_converted.
       Definition mul_converted
               n1 n2 (* lengths in original format *)
               m1 m2 (* lengths in converted format *)
@@ -1631,104 +1672,63 @@ Module MulConverted.
         let p3_a := Associational.mul p1_a p2_a in
         from_associational idxs n3 p3_a.
 
-      Hint Rewrite
-           @Rows.eval_from_associational
-           @Associational.eval_carry
-           @Associational.eval_mul
-           @Positional.eval_to_associational
-           @BaseConversion.eval_convert_bases using solve [auto using Z.positive_is_nonzero] : push_eval.
-
-      Ltac push_eval := intros; autorewrite with push_eval; auto with zarith.
-
-      Lemma eval_carries p idxs :
-        Associational.eval (fold_right (fun i acc => Associational.carry (w' i) (w' (S i) / w' i) acc) p idxs) =
-        Associational.eval p.
-      Proof. apply fold_right_invariant; push_eval. Qed.
-      Hint Rewrite eval_carries: push_eval.
-
-      Lemma eval_to_associational n m p :
-        m <> 0%nat -> length p = n ->
-        Associational.eval (to_associational n m p) = Positional.eval w n p.
-      Proof. cbv [to_associational]; push_eval. Qed.
-      Hint Rewrite eval_to_associational using solve [push_eval; distr_length] : push_eval.
-
-      Lemma eval_from_associational idxs n p :
-        n <> 0%nat -> 0 <= Associational.eval p < w n ->
-        Positional.eval w n (from_associational idxs n p) = Associational.eval p.
-      Proof.
-        cbv [from_associational]; intros.
-        rewrite Rows.flatten_mod by eauto using Rows.length_from_associational.
-        push_eval.
-      Qed.
-      Hint Rewrite eval_from_associational using solve [push_eval; distr_length] : push_eval.
-
       Lemma eval_mul_converted n1 n2 m1 m2 n3 idxs p1 p2 (_:n3<>0%nat) (_:m1<>0%nat) (_:m2<>0%nat):
         length p1 = n1 -> length p2 = n2 ->
-        0 <= (Positional.eval w n1 p1 * Positional.eval w n2 p2) < w n3 ->
-        Positional.eval w n3 (mul_converted n1 n2 m1 m2 n3 idxs p1 p2) = (Positional.eval w n1 p1) * (Positional.eval w n2 p2).
+        0 <= (Positional.eval sw n1 p1 * Positional.eval sw n2 p2) < sw n3 ->
+        Positional.eval sw n3 (mul_converted n1 n2 m1 m2 n3 idxs p1 p2) = (Positional.eval sw n1 p1) * (Positional.eval sw n2 p2).
       Proof.  cbv [mul_converted]; push_eval. Qed.
       Hint Rewrite eval_mul_converted : push_eval.
 
-      Lemma from_associational_partitions n idxs p  (_:n<>0%nat):
-        forall i, (i < n)%nat ->
-        nth_default 0 (from_associational idxs n p) i = (Associational.eval p) mod (w (S i)) / w i.
-      Proof.
-        intros; cbv [from_associational].
-        rewrite Rows.flatten_partitions with (n:=n) by (eauto using Rows.length_from_associational; omega).
-        push_eval.
-      Qed.
-
       Lemma mul_converted_partitions n1 n2 m1 m2 n3 idxs p1 p2  (_:n3<>0%nat) (_:m1<>0%nat) (_:m2<>0%nat):
         length p1 = n1 -> length p2 = n2 ->
-        forall i, (i < n3)%nat ->
-        nth_default 0 (mul_converted n1 n2 m1 m2 n3 idxs p1 p2) i = (Positional.eval w n1 p1 * Positional.eval w n2 p2) mod (w (S i)) / w i.
-      Proof.
-        intros; cbv [mul_converted].
-        rewrite from_associational_partitions by auto. push_eval.
-      Qed.
-
-      Lemma from_associational_eq n idxs p  (_:n<>0%nat):
-        from_associational idxs n p = Rows.partition w n (Associational.eval p).
-      Proof.
-        intros. cbv [from_associational].
-        rewrite Rows.flatten_partitions' with (n:=n) by eauto using Rows.length_from_associational.
-        push_eval.
-      Qed.
-        
-      (* TODO: convert all _partitions proofs to this form? *)
-      Lemma mul_converted_eq n1 n2 m1 m2 n3 idxs p1 p2  (_:n3<>0%nat) (_:m1<>0%nat) (_:m2<>0%nat):
-        length p1 = n1 -> length p2 = n2 ->
-        mul_converted n1 n2 m1 m2 n3 idxs p1 p2 = Rows.partition w n3 (Positional.eval w n1 p1 * Positional.eval w n2 p2).
+        mul_converted n1 n2 m1 m2 n3 idxs p1 p2 = Rows.partition sw n3 (Positional.eval sw n1 p1 * Positional.eval sw n2 p2).
       Proof.
         intros; cbv [mul_converted].
         rewrite from_associational_eq by auto. push_eval.
       Qed.
+    End mul_converted.
+  End BaseConversion.
 
-      Section aligned.
-        Context (log_w'_w : nat) (Hlog_w'_w : forall i, (w' i) ^ Z.of_nat log_w'_w = w i).
-        Context (n n' nout : nat) (Hn : n <> 0%nat) (Hn' : n' <> 0%nat) (Hnout : nout <> 0%nat).
-        
-        (* carry chain that aligns terms in the intermediate weight with the final weight *)
-        Definition aligned_carries := (map (fun i => ((log_w'_w * (i + 1)) - 1))%nat (seq 0 nout)).
-        
-        Definition from_associational_aligned := from_associational aligned_carries nout.
-        
-        (* assumes both inputs have the same length *)
-        Definition mul_aligned := mul_converted n n n' n' nout aligned_carries.
+  (* multiply two (n*k)-bit numbers by converting them to n k-bit limbs each, multiplying, then converting back *)
+  Section widemul.
+    Context (dw : nat -> Z) (n : nat) (n_nz : n <> 0%nat).
+    Context (dw_0 : dw 0%nat = 1)
+            (dw_pos : forall i, dw i > 0)
+            (dw_multiples : forall i, dw (S i) mod dw i = 0)
+            (dw_divides : forall i, dw (S i) / dw i > 0).
+    Context (nout : nat) (nout_nz : nout <> 0%nat). (* this is always 2, but reification has trouble if it's a constant *)
+    Let sw i := (dw i) ^ Z.of_nat n.
 
-        Lemma mul_aligned_eq p1 p2 :
-          length p1 = n -> length p2 = n ->
-          mul_aligned p1 p2 = Rows.partition w nout (Positional.eval w n p1 * Positional.eval w n p2).
-        Proof. cbv [mul_aligned aligned_carries]. auto using mul_converted_eq. Qed.
+    Hint Resolve Z.gt_lt Z.positive_is_nonzero Nat2Z.is_nonneg.
+    (* TODO : There has got to be a cleaner way to do weight functions *)
+    Lemma sw_0 : sw 0 = 1.
+    Proof. subst sw; cbv beta. rewrite dw_0. auto using Z.pow_1_l. Qed.
+    Lemma sw_pos : forall i, sw i > 0.
+    Proof. subst sw; intros; apply Z.lt_gt. Z.zero_bounds. Qed.
+    Lemma sw_nz : forall i, sw i <> 0.
+    Proof. auto using sw_pos. Qed.
+    Lemma sw_multiples : forall i, sw (S i) mod sw i = 0.
+    Proof.
+      subst sw; cbv beta; intros.
+      rewrite Saturated.weight_div_mod with (weight := dw) (j:=S i) (i:=i) by auto.
+      rewrite Z.pow_mul_l.
+      push_Zmod. autorewrite with zsimplify. reflexivity.
+    Qed.
+    Lemma sw_divides : forall i, sw (S i) / sw i > 0.
+    Proof. intros; apply Z.div_positive_gt_0; auto using sw_pos, sw_multiples. Qed.
+    Hint Resolve sw_0 sw_pos sw_nz sw_multiples sw_divides.
 
-        Lemma eval_mul_aligned p1 p2 :
-          length p1 = n -> length p2 = n ->
-          0 <= Positional.eval w n p1 * Positional.eval w n p2 < w nout ->
-          Positional.eval w nout (mul_aligned p1 p2) = Positional.eval w n p1 * Positional.eval w n p2.
-        Proof. cbv [mul_aligned aligned_carries]. auto using eval_mul_converted. Qed.
-      End aligned.
-  End mul_converted.
-End MulConverted.
+    Definition widemul a b := mul_converted sw dw 1 1 n n nout (aligned_carries n nout) [a] [b].
+
+    Lemma widemul_partitions a b :
+      widemul a b = Rows.partition sw nout (a * b).
+    Proof.
+      cbv [widemul].
+      rewrite mul_converted_partitions by auto with zarith.
+      cbn; rewrite sw_0; ring_simplify_subterms. reflexivity.
+    Qed.
+  End widemul.
+End BaseConversion.
 
 Module Import MOVEME.
   Fixpoint fold_andb_map {A B} (f : A -> B -> bool) (ls1 : list A) (ls2 : list B)
@@ -7810,6 +7810,7 @@ Module MontgomeryReduction.
       := weight_multiples _ _ half_log2R_good.
     Let w_mul_divides : forall i : nat, w_mul (S i) / w_mul i > 0
       := weight_divides _ _ half_log2R_good.
+(*
     Let w_0 : w 0%nat = 1 := weight_0 _ _.
     Let w_nonzero : forall i, w i <> 0
       := weight_nz _ _ log2R_good.
@@ -7820,14 +7821,13 @@ Module MontgomeryReduction.
     Let w_divides : forall i : nat, w (S i) / w i > 0
       := weight_divides _ _ log2R_good.
     Let w_1_gt1 : w 1 > 1 := weight_1_gt_1 _ _ log2R_good.
+*)
     Let w_mul_1_gt1 : w_mul 1 > 1 := weight_1_gt_1 _ _ half_log2R_good.
     Context (nout : nat) (Hnout : nout = 2%nat).
 
-    Definition widemul a b := MulConverted.mul_aligned w w_mul n 1%nat n nout [a] [b].
-
     Definition montred' (lo_hi : (Z * Z)) :=
-      dlet_nd y := nth_default 0 (widemul (fst lo_hi) N') 0  in
-      dlet_nd t1_t2 := widemul y N in
+      dlet_nd y := nth_default 0 (BaseConversion.widemul w_mul n nout (fst lo_hi) N') 0  in
+      dlet_nd t1_t2 := (BaseConversion.widemul w_mul n nout y N) in
       dlet_nd lo'_carry := Z.add_get_carry_full R (fst lo_hi) (nth_default 0 t1_t2 0) in
       dlet_nd hi'_carry := Z.add_with_get_carry_full R (snd lo'_carry) (snd lo_hi) (nth_default 0 t1_t2 1) in
       dlet_nd y' := Z.zselect (snd hi'_carry) 0 N in
@@ -7841,7 +7841,7 @@ Module MontgomeryReduction.
       rewrite Z.pow_mul_r, R_two_pow by omega; reflexivity.
     Qed.
 
-    Local Ltac change_weight := rewrite !Hw, ?Z.pow_0_r, ?Z.pow_1_r, ?Z.pow_2_r in *.
+    Local Ltac change_weight := rewrite ?w_mul_pown, !Hw, ?Z.pow_0_r, ?Z.pow_1_r, ?Z.pow_2_r in *.
     Local Ltac solve_range :=
       repeat match goal with
              | _ => progress change_weight
@@ -7855,9 +7855,10 @@ Module MontgomeryReduction.
              end.
 
     Lemma widemul_correct x y :
-      0 <= x * y < w 2 -> widemul x y = [(x * y) mod R; (x * y) / R].
+      0 <= x * y < w 2 -> BaseConversion.widemul w_mul n nout x y = [(x * y) mod R; (x * y) / R].
     Proof.
-      intros; cbv [widemul]. rewrite MulConverted.mul_aligned_eq by (auto; distr_length).
+      intros.
+      rewrite BaseConversion.widemul_partitions by (auto; omega).
       subst nout. cbn. change_weight.
       autorewrite with zsimplify.
       Z.rewrite_mod_small. reflexivity.
